Add incremental forward reasoning
We introduce a new, incremental forward reasoning algorithm. "Incremental"
means that the algorithm takes advantage of similarities between parent
and child goals, i.e. a forward rule that was run on the parent goal is
not re-run on the child goal unless the hypotheses that the rule was
applied to have changed or disappeared.

The new algorithm is enabled by default and can be toggled with the
`aesop.dev.statefulForward` option.

Breaking changes:

- Forward rules (including destruct rules) always use `reducible`
  transparency and no longer support custom indexing modes.
- `destruct` rules no longer clear non-propositional hypotheses.

See also
https://leanprover.zulipchat.com/#narrow/channel/270676-lean4/topic/Upcoming.20changes.20to.20Aesop.20forward.20rules

See the `forward-code` branch for the history of this feature.

closes #111

Aesop/RuleTac/Forward.lean
@@ -4,39 +4,33 @@ Released under Apache 2.0 license as described in the file LICENSE.
 Authors: Jannis Limperg
 -/
 
+import Aesop.Forward.Match
 import Aesop.RuleTac.Basic
 import Aesop.RuleTac.ElabRuleTerm
-import Batteries.Lean.Meta.UnusedNames
-import Aesop.Script.SpecificTactics
 import Aesop.RuleTac.Forward.Basic
+import Aesop.Script.SpecificTactics
+import Batteries.Lean.Meta.UnusedNames
 
 open Lean
 open Lean.Meta
 
 namespace Aesop.RuleTac
 
-partial def makeForwardHyps (e : Expr) (pat? : Option RulePattern)
-    (patInst : RulePatternInstantiation) (immediate : UnorderedArraySet Nat)
-    (maxDepth? : Option Nat) (forwardHypData : ForwardHypData) :
-    MetaM (Array (Expr × Nat) × Array FVarId) :=
+partial def makeForwardHyps (e : Expr) (patSubst? : Option Substitution)
+    (immediate : UnorderedArraySet PremiseIndex) (maxDepth? : Option Nat)
+    (forwardHypData : ForwardHypData) (existingHypTypes : PHashSet RPINF) :
+    BaseM (Array (Expr × Nat) × Array FVarId) :=
   withNewMCtxDepth (allowLevelAssignments := true) do
     let type ← inferType e
-    let (argMVars, binderInfos, patInstantiatedMVars) ←
-      if let some pat := pat? then
-        let (argMVars, binderInfos, _, patInstantiatedMVars) ←
-          pat.openRuleType patInst type
-        pure (argMVars, binderInfos, patInstantiatedMVars)
-      else
-        let (argMVars, binderInfos, _) ← forallMetaTelescopeReducing type
-        pure (argMVars, binderInfos, ∅)
-    let app := mkAppN e argMVars
+    let (argMVars, binderInfos, _) ← openRuleType patSubst? e
+    let app := mkAppN e (argMVars.map .mvar)
     let mut instMVars := Array.mkEmpty argMVars.size
     let mut immediateMVars := Array.mkEmpty argMVars.size
     for h : i in [:argMVars.size] do
-      let mvarId := argMVars[i].mvarId!
-      if patInstantiatedMVars.contains mvarId then
+      let mvarId := argMVars[i]
+      if ← mvarId.isAssignedOrDelayedAssigned then
         continue
-      if immediate.contains i then
+      if immediate.contains ⟨i⟩ then
         immediateMVars := immediateMVars.push mvarId
       else if binderInfos[i]!.isInstImplicit then
         instMVars := instMVars.push mvarId
@@ -47,10 +41,26 @@ partial def makeForwardHyps (e : Expr) (pat? : Option RulePattern)
     loop (app : Expr) (instMVars : Array MVarId) (immediateMVars : Array MVarId)
         (i : Nat) (proofsAcc : Array (Expr × Nat)) (currentMaxHypDepth : Nat)
         (currentUsedHyps : Array FVarId) (usedHypsAcc : Array FVarId)
-        (proofTypesAcc : Std.HashSet Expr) :
-        MetaM (Array (Expr × Nat) × Array FVarId × Std.HashSet Expr) := do
-      if h : i < immediateMVars.size then
-        let mvarId := immediateMVars[i]
+        (proofTypesAcc : Std.HashSet RPINF) :
+        BaseM (Array (Expr × Nat) × Array FVarId × Std.HashSet RPINF) := do
+      if h : immediateMVars.size > 0 ∧ i < immediateMVars.size then
+        -- We go through the immediate mvars back to front. This is more
+        -- efficient because assigning later mvars may already determine the
+        -- assignments of earlier mvars.
+        let mvarId := immediateMVars[immediateMVars.size - 1 - i]
+        if ← mvarId.isAssignedOrDelayedAssigned then
+          -- If the mvar is already assigned, we still need to update and check
+          -- the hyp depth.
+          let mut currentMaxHypDepth := currentMaxHypDepth
+          let (_, fvarIds) ← (← instantiateMVars (.mvar mvarId)).collectFVars |>.run {}
+          for fvarId in fvarIds.fvarIds do
+            let hypDepth := forwardHypData.depths.getD fvarId 0
+            currentMaxHypDepth := max currentMaxHypDepth hypDepth
+          if let some maxDepth := maxDepth? then
+            if currentMaxHypDepth + 1 > maxDepth then
+              return (proofsAcc, usedHypsAcc, proofTypesAcc)
+          return ← loop app instMVars immediateMVars (i + 1) proofsAcc
+            currentMaxHypDepth currentUsedHyps usedHypsAcc proofTypesAcc
         let type ← mvarId.getType
         (← getLCtx).foldlM (init := (proofsAcc, usedHypsAcc, proofTypesAcc)) λ s@(proofsAcc, usedHypsAcc, proofTypesAcc) ldecl => do
           if ldecl.isImplementationDetail then
@@ -74,10 +84,9 @@ partial def makeForwardHyps (e : Expr) (pat? : Option RulePattern)
             let inst ← synthInstance (← instMVar.getType)
             instMVar.assign inst
         let proof := (← abstractMVars app).expr
-        let type ← instantiateMVars (← inferType proof)
-        let redundant ←
-          pure (proofTypesAcc.contains type) <||>
-          forwardHypData.containsTypeUpToIds type
+        let type ← rpinf (← inferType proof)
+        let redundant :=
+          proofTypesAcc.contains type || existingHypTypes.contains type
         if redundant then
           return (proofsAcc, usedHypsAcc, proofTypesAcc)
         else
@@ -87,10 +96,10 @@ partial def makeForwardHyps (e : Expr) (pat? : Option RulePattern)
           let usedHypsAcc := usedHypsAcc ++ currentUsedHyps
           return (proofsAcc, usedHypsAcc, proofTypesAcc)
 
-def assertForwardHyp (goal : MVarId) (hyp : Hypothesis) (depth : Nat)
-    (md : TransparencyMode) : ScriptM (FVarId × MVarId) := do
+def assertForwardHyp (goal : MVarId) (hyp : Hypothesis) (depth : Nat) :
+    ScriptM (FVarId × MVarId) := do
   withScriptStep goal (λ (_, g) => #[g]) (λ _ => true) tacticBuilder do
-  withTransparency md do
+  withReducible do
     let hyp := {
       hyp with
       binderInfo := .default
@@ -106,25 +115,29 @@ def assertForwardHyp (goal : MVarId) (hyp : Hypothesis) (depth : Nat)
       | throwError "aesop: internal error in assertForwardHyp: unexpected number of asserted fvars"
     return (fvarId, goal)
 where
-  tacticBuilder _ := Script.TacticBuilder.assertHypothesis goal hyp md
+  tacticBuilder _ := Script.TacticBuilder.assertHypothesis goal hyp .reducible
 
-def applyForwardRule (goal : MVarId) (e : Expr) (pat? : Option RulePattern)
-    (patInsts : Std.HashSet RulePatternInstantiation)
-    (immediate : UnorderedArraySet Nat) (clear : Bool)
-    (md : TransparencyMode) (maxDepth? : Option Nat) : ScriptM Subgoal :=
-  withTransparency md $ goal.withContext do
+def applyForwardRule (goal : MVarId) (e : Expr)
+    (patSubsts? : Option (Std.HashSet Substitution))
+    (immediate : UnorderedArraySet PremiseIndex) (clear : Bool)
+    (maxDepth? : Option Nat) (existingHypTypes : PHashSet RPINF) :
+    ScriptM Subgoal :=
+  withReducible $ goal.withContext do
+    let initialGoal := goal
     let forwardHypData ← getForwardHypData
     let mut newHypProofs := #[]
     let mut usedHyps := ∅
-    if pat?.isSome then
-      for patInst in patInsts do
+    if let some patSubsts := patSubsts? then
+      for patSubst in patSubsts do
         let (newHypProofs', usedHyps') ←
-          makeForwardHyps e pat? patInst immediate maxDepth? forwardHypData
+          makeForwardHyps e patSubst immediate maxDepth? forwardHypData
+            existingHypTypes
         newHypProofs := newHypProofs ++ newHypProofs'
         usedHyps := usedHyps ++ usedHyps'
     else
       let (newHypProofs', usedHyps') ←
-        makeForwardHyps e pat? .empty immediate maxDepth? forwardHypData
+        makeForwardHyps e none immediate maxDepth? forwardHypData
+          existingHypTypes
       newHypProofs := newHypProofs'
       usedHyps := usedHyps'
     usedHyps :=
@@ -139,53 +152,69 @@ def applyForwardRule (goal : MVarId) (e : Expr) (pat? : Option RulePattern)
     let mut goal := goal
     let mut addedFVars := ∅
     for (newHyp, depth) in newHyps do
-      let (fvarId, goal') ← assertForwardHyp goal newHyp depth md
+      let (fvarId, goal') ← assertForwardHyp goal newHyp depth
       goal := goal'
       addedFVars := addedFVars.insert fvarId
     let mut diff := {
+      oldGoal := initialGoal
+      newGoal := goal
       addedFVars
       removedFVars := ∅
-      fvarSubst := ∅
+      targetChanged := .false
     }
     if clear then
-      let (goal', removedFVars) ← tryClearManyS goal usedHyps
+      let usedPropHyps ← goal.withContext do
+        usedHyps.filterM λ fvarId => isProof (.fvar fvarId)
+      let (goal', removedFVars) ← tryClearManyS goal usedPropHyps
       let removedFVars := removedFVars.foldl (init := ∅) λ set fvarId =>
         set.insert fvarId
-      diff := { diff with removedFVars := removedFVars }
       goal := goal'
-    return { mvarId := goal, diff }
+      diff := { diff with newGoal := goal, removedFVars }
+    return { diff }
   where
     err {α} : MetaM α := throwError
       "found no instances of {e} (other than possibly those which had been previously added by forward rules)"
 
 @[inline]
-def forwardExpr (e : Expr) (pat? : Option RulePattern)
-    (immediate : UnorderedArraySet Nat) (clear : Bool) (md : TransparencyMode) :
-    RuleTac :=
+def forwardExpr (e : Expr) (immediate : UnorderedArraySet PremiseIndex)
+    (clear : Bool) : RuleTac :=
   SingleRuleTac.toRuleTac λ input => input.goal.withContext do
     let (goal, steps) ←
-      applyForwardRule input.goal e pat? input.patternInstantiations immediate
-        (clear := clear) md input.options.forwardMaxDepth? |>.run
+      applyForwardRule input.goal e input.patternSubsts? immediate
+        (clear := clear) input.options.forwardMaxDepth? input.hypTypes
+      |>.run
     return (#[goal], steps, none)
 
-def forwardConst (decl : Name) (pat? : Option RulePattern)
-    (immediate : UnorderedArraySet Nat) (clear : Bool) (md : TransparencyMode) :
-    RuleTac := λ input => do
+def forwardConst (decl : Name) (immediate : UnorderedArraySet PremiseIndex)
+    (clear : Bool) : RuleTac := λ input => do
   let e ← mkConstWithFreshMVarLevels decl
-  forwardExpr e pat? immediate (clear := clear) md input
+  forwardExpr e immediate (clear := clear) input
 
-def forwardTerm (stx : Term) (pat? : Option RulePattern)
-    (immediate : UnorderedArraySet Nat) (clear : Bool) (md : TransparencyMode) :
-    RuleTac := λ input =>
+def forwardTerm (stx : Term) (immediate : UnorderedArraySet PremiseIndex)
+    (clear : Bool) : RuleTac := λ input =>
   input.goal.withContext do
     let e ← elabRuleTermForApplyLikeMetaM input.goal stx
-    forwardExpr e pat? immediate (clear := clear) md input
+    forwardExpr e immediate (clear := clear) input
 
-def forward (t : RuleTerm) (pat? : Option RulePattern)
-    (immediate : UnorderedArraySet Nat) (clear : Bool) (md : TransparencyMode) :
-    RuleTac :=
+def forward (t : RuleTerm) (immediate : UnorderedArraySet PremiseIndex)
+    (clear : Bool) : RuleTac :=
   match t with
-  | .const decl => forwardConst decl pat? immediate clear md
-  | .term tm => forwardTerm tm pat? immediate clear md
+  | .const decl => forwardConst decl immediate clear
+  | .term tm => forwardTerm tm immediate clear
+
+def forwardMatch (m : ForwardRuleMatch) :
+    RuleTac := SingleRuleTac.toRuleTac λ input => do
+  let skip type := input.hypTypes.contains type
+  let (some (goal, hyp, removedFVars), steps) ←
+    m.apply input.goal (some skip) |>.run
+    | throwError "hyp already exists or synthesis of instance arguments failed"
+  let diff := {
+    oldGoal := input.goal
+    newGoal := goal
+    addedFVars := {hyp}
+    targetChanged := .false
+    removedFVars := .ofArray removedFVars
+  }
+  return (#[{ diff }], some steps, none)
 
 end Aesop.RuleTac
