Aesop/Saturate.lean
@@ -4,12 +4,16 @@ Released under Apache 2.0 license as described in the file LICENSE.
 Authors: Jannis Limperg
 -/
 
+import Aesop.Forward.State.ApplyGoalDiff
+import Aesop.Forward.State.Initial
 import Aesop.RuleSet
 import Aesop.RuleTac
 import Aesop.Search.Expansion.Basic
 import Aesop.Script.Check
+import Batteries.Data.BinomialHeap.Basic
 
 open Lean Lean.Meta
+open Batteries (BinomialHeap)
 
 namespace Aesop
 
@@ -18,16 +22,31 @@ def isForwardOrDestructRuleName (n : RuleName) : Bool :=
 
 structure SaturateM.Context where
   options : Aesop.Options'
+  deriving Inhabited
 
-abbrev SaturateM := ReaderT SaturateM.Context ScriptM
+structure SaturateM.State where
+  rulePatternCache : RulePatternCache := {}
+  rpinfCache : RPINFCache := ∅
+  deriving Inhabited
+
+abbrev SaturateM :=
+  ReaderT SaturateM.Context $ StateRefT SaturateM.State $ ScriptT BaseM
+
+namespace SaturateM
+
+def run (options : Aesop.Options') (x : SaturateM α) :
+    MetaM (α × Array Script.LazyStep) :=
+  ReaderT.run x { options } |>.run' {} |>.run.run
+
+end SaturateM
 
 def getSingleGoal [Monad m] [MonadError m] (o : RuleTacOutput) :
-    m (MVarId × Meta.SavedState × Option (Array Script.LazyStep)) := do
+    m (GoalDiff × Meta.SavedState × Option (Array Script.LazyStep)) := do
   let #[app] := o.applications
     | throwError "rule produced more than one rule application"
   let #[goal] := app.goals
     | throwError "rule did not produce exactly one subgoal"
-  return (goal.mvarId, app.postState, app.scriptSteps?)
+  return (goal.diff, app.postState, app.scriptSteps?)
 
 initialize
   registerTraceClass `saturate
@@ -35,47 +54,54 @@ initialize
 partial def saturateCore (rs : LocalRuleSet) (goal : MVarId) : SaturateM MVarId :=
   withExceptionPrefix "saturate: internal error: " do
   goal.checkNotAssigned `saturate
-  go goal
+  -- We use the forward state only to track the hypotheses present in the goal.
+  let (fs, _) ← rs.mkInitialForwardState goal
+  go goal fs
 where
-  go (goal : MVarId) : SaturateM MVarId :=
+  go (goal : MVarId) (fs : ForwardState) : SaturateM MVarId :=
     withIncRecDepth do
     trace[saturate] "goal {goal.name}:{indentD goal}"
     let mvars := UnorderedArraySet.ofHashSet $ ← goal.getMVarDependencies
     let preState ← show MetaM _ from saveState
-    if let some goal ← tryNormRules goal mvars preState then
-      return ← go goal
-    else if let some goal ← trySafeRules goal mvars preState then
-      return ← go goal
+    if let some diff ← tryNormRules goal mvars preState fs.hypTypes then
+      let (fs, _) ← fs.applyGoalDiff rs diff
+      return ← go diff.newGoal fs
+    else if let some diff ← trySafeRules goal mvars preState fs.hypTypes then
+      let (fs, _) ← fs.applyGoalDiff rs diff
+      return ← go diff.newGoal fs
     else
       clearForwardImplDetailHyps goal
 
   tryNormRules (goal : MVarId) (mvars : UnorderedArraySet MVarId)
-      (preState : Meta.SavedState) : SaturateM (Option MVarId) :=
+      (preState : Meta.SavedState) (hypTypes : PHashSet RPINF) :
+      SaturateM (Option GoalDiff) :=
     withTraceNode `saturate (λ res => return m!"{exceptOptionEmoji res} trying normalisation rules") do
       let matchResults ←
         withTraceNode `saturate (λ res => return m!"{exceptEmoji res} selecting normalisation rules") do
-        rs.applicableNormalizationRulesWith goal
+        rs.applicableNormalizationRulesWith ∅ goal
           (include? := (isForwardOrDestructRuleName ·.name))
-      runFirstRule goal mvars preState matchResults
+      runFirstRule goal mvars preState matchResults hypTypes
 
   trySafeRules (goal : MVarId) (mvars : UnorderedArraySet MVarId)
-      (preState : Meta.SavedState) : SaturateM (Option MVarId) :=
+      (preState : Meta.SavedState) (hypTypes : PHashSet RPINF) :
+      SaturateM (Option GoalDiff) :=
     withTraceNode `saturate (λ res => return m!"{exceptOptionEmoji res} trying safe rules") do
       let matchResults ←
         withTraceNode `saturate (λ res => return m!"{exceptEmoji res} selecting safe rules") do
-        rs.applicableSafeRulesWith goal
+        rs.applicableSafeRulesWith ∅ goal
           (include? := (isForwardOrDestructRuleName ·.name))
-      runFirstRule goal mvars preState matchResults
+      runFirstRule goal mvars preState matchResults hypTypes
 
   runRule {α} (goal : MVarId) (mvars : UnorderedArraySet MVarId)
-      (preState : Meta.SavedState) (matchResult : IndexMatchResult (Rule α)) :
-      SaturateM (Option (MVarId × Option (Array Script.LazyStep))) := do
+      (preState : Meta.SavedState) (matchResult : IndexMatchResult (Rule α))
+      (hypTypes : PHashSet RPINF) :
+      SaturateM (Option (GoalDiff × Option (Array Script.LazyStep))) := do
     withTraceNode `saturate (λ res => return m!"{exceptOptionEmoji res} running rule {matchResult.rule.name}") do
     let input := {
       indexMatchLocations := matchResult.locations
-      patternInstantiations := matchResult.patternInstantiations
+      patternSubsts? := matchResult.patternSubsts?
       options := (← read).options
-      goal, mvars
+      hypTypes, goal, mvars
     }
     let tacResult ←
       runRuleTac matchResult.rule.tac.run matchResult.rule.name preState input
@@ -84,32 +110,98 @@ where
       trace[saturate] exc.toMessageData
       return none
     | .inr output =>
-      let (goal, postState, scriptSteps?) ← getSingleGoal output
+      let (diff, postState, scriptSteps?) ← getSingleGoal output
       postState.restore
-      return (goal, scriptSteps?)
+      return (diff, scriptSteps?)
 
   runFirstRule {α} (goal : MVarId) (mvars : UnorderedArraySet MVarId)
       (preState : Meta.SavedState)
-      (matchResults : Array (IndexMatchResult (Rule α))) :
-      SaturateM (Option MVarId) := do
+      (matchResults : Array (IndexMatchResult (Rule α)))
+      (hypTypes : PHashSet RPINF) : SaturateM (Option GoalDiff) := do
     for matchResult in matchResults do
-      if let some (goal, scriptSteps?) ← runRule goal mvars preState matchResult then
+      let ruleResult? ← runRule goal mvars preState matchResult hypTypes
+      if let some (diff, scriptSteps?) := ruleResult? then
         if (← read).options.generateScript then
           let some scriptSteps := scriptSteps?
             | throwError "rule '{matchResult.rule.name}' does not support script generation (saturate?)"
           recordScriptSteps scriptSteps
-        return some goal
+        return some diff
     return none
+
+namespace Stateful
+
+abbrev Queue := BinomialHeap ForwardRuleMatch ForwardRuleMatch.le
+
+partial def saturateCore (rs : LocalRuleSet) (goal : MVarId)
+    (options : Options') : SaturateM MVarId :=
+  withExceptionPrefix "saturate: internal error: " do
+  goal.withContext do
+    goal.checkNotAssigned `saturate
+    let (fs, ruleMatches) ← rs.mkInitialForwardState goal
+    let queue := ruleMatches.foldl (init := ∅) λ queue m => queue.insert m
+    go ∅ fs queue ∅ goal
+where
+  go (hypDepths : Std.HashMap FVarId Nat) (fs : ForwardState) (queue : Queue)
+      (erasedHyps : Std.HashSet FVarId) (goal : MVarId) : SaturateM MVarId := do
+    withIncRecDepth do
+    goal.withContext do
+      if let some (m, queue) := queue.deleteMin then
+        if m.rule.name.phase == .unsafe || m.anyHyp erasedHyps.contains then
+          return ← go hypDepths fs queue erasedHyps goal
+        trace[saturate] "goal:{indentD goal}"
+        let oldGoal := goal
+        let some (goal, hyp, removedHyps) ←
+          m.apply goal (skip? := some (fs.hypTypes.contains ·))
+          | return ← go hypDepths fs queue erasedHyps goal
+        goal.withContext do
+          -- TODO use applyGoalDiff
+          let fs ← removedHyps.foldlM (init := fs) λ fs h => do
+            let type ← oldGoal.withContext do rpinf (← h.getType)
+            return fs.eraseHyp h type
+          let type ← hyp.getType
+          let erasedHyps := erasedHyps.insertMany removedHyps
+          let mut depth := 0
+          let mut hypDepths := hypDepths
+          let maxDepth? := options.forwardMaxDepth?
+          if maxDepth?.isSome then
+            depth := 1 + m.foldHyps (init := 0) λ depth h =>
+              max depth (hypDepths[h]?.getD 0)
+            hypDepths := hypDepths.insert hyp depth
+          trace[saturate] "added hyp (depth {depth}) {Expr.fvar hyp} : {type}"
+          if maxDepth?.isSome && depth ≥ maxDepth?.get! then
+            go hypDepths fs queue erasedHyps goal
+          else
+            let rules ← rs.applicableForwardRules type
+            let patInsts ←
+              rs.forwardRulePatternSubstsInLocalDecl (← hyp.getDecl)
+            let (fs, ruleMatches) ←
+              fs.addHypWithPatSubsts goal hyp rules patInsts
+            let queue :=
+              ruleMatches.foldl (init := queue) λ queue m => queue.insert m
+            go hypDepths fs queue erasedHyps goal
+      else
+        return goal
+
+end Stateful
+
+def saturateMain (rs : LocalRuleSet) (goal : MVarId) (options : Aesop.Options') :
+    MetaM (MVarId × Array Script.LazyStep) := do
+  let doSaturate :=
+    if aesop.dev.statefulForward.get (← getOptions) then
+      Stateful.saturateCore rs goal options
+    else
+      saturateCore rs goal
+  doSaturate.run options
 
 def saturate (rs : LocalRuleSet) (goal : MVarId) (options : Aesop.Options') :
     MetaM MVarId := do
   if ! options.generateScript then
-    (·.fst) <$> (saturateCore rs goal |>.run { options } |>.run)
+    (·.fst) <$> saturateMain rs goal options
   else
     let preState ← saveState
     let tacticState ← Script.TacticState.mkInitial goal
     let preGoal := goal
-    let (goal, steps) ← saturateCore rs goal |>.run { options } |>.run
+    let (goal, steps) ← saturateMain rs goal options
     let options ← options.toOptions'
     if options.generateScript then
       let uscript : Script.UScript ← steps.mapM (·.toStep)
