AesopTest/Forward.lean
@@ -1,5 +1,5 @@
 /-
-Copyright (c) 2021 Jannis Limperg. All rights reserved.
+Copyright (c) 2024 Jannis Limperg. All rights reserved.
 Released under Apache 2.0 license as described in the file LICENSE.
 Authors: Jannis Limperg
 -/
@@ -10,95 +10,45 @@ set_option aesop.check.all true
 set_option aesop.smallErrorMessages true
 set_option pp.mvars false
 
-open Aesop Lean Lean.Meta Lean.Elab.Tactic
-
-/-! # Unit tests for the MetaM tactic that implements forward rules -/
-
-syntax (name := forward) "t_forward " ident (" [" ident* "]")? : tactic
-syntax (name := elim)    "t_elim "    ident (" [" ident* "]")? : tactic
-
-def forwardTac (goal : MVarId) (id : Ident) (immediate : Option (Array Syntax))
-    (clear : Bool) (md : TransparencyMode) : MetaM (List MVarId) := do
-  let userName := id.getId
-  let ldecl ← getLocalDeclFromUserName userName
-  let immediate ← RuleBuilder.getImmediatePremises ldecl.type none md
-    (immediate.map (·.map (·.getId)))
-  let (goal, _) ←
-    RuleTac.applyForwardRule goal (mkFVar ldecl.fvarId) none ∅ immediate clear
-      md (maxDepth? := none) |>.run
-  return [goal.mvarId]
-
-@[tactic forward]
-def evalForward : Tactic
-  | `(tactic| t_forward $t:ident $[[ $immediate:ident* ]]?) =>
-    liftMetaTactic (forwardTac · t immediate (clear := false) .default)
-  | _ => unreachable!
-
-@[tactic elim]
-def evalElim : Tactic
-  | `(tactic| t_elim $t:ident $[[ $immediate:ident* ]]?) =>
-    liftMetaTactic (forwardTac · t immediate (clear := true) .default)
-  | _ => unreachable!
-
-example (rule : (a : α) → (b : β) → γ) (h₁ : α) (h₂ : β) : γ := by
-  t_forward rule [a b]
-  assumption
-
-example {P Q R : α → Type} (rule : ∀ a (p : P a) (q : Q a), R a)
-    (h₁ : P a) (h₁' : P a) (h₂ : Q a) (h₃ : P b) (h₄ : Q c) : R a := by
-  t_forward rule [p q]
-  assumption
-
-example {P Q R : α → Type} (rule : ∀ a (p : P a) (q : Q a), R a)
-    (h₁ : P a) (h₁' : P a) (h₂ : Q a) (h₃ : P b) (h₄ : Q c) : R a := by
-  t_forward rule
-  assumption
-
-example {P Q R : α → Type} (rule : ∀ a (p : P a) (q : Q a), R a)
-    (h₁ : P a) (h₂ : P b) : (Q a → R a) × (Q b → R b) := by
-  t_forward rule [p]
-  exact (by assumption, by assumption)
-
-example (rule : ∀ α β, α ∧ β → α) (h : P ∧ Q ∧ R) : P := by
-  t_elim rule
-  assumption
-
-/-! # Tests for the `forward` and `saturate` tactics -/
-
-/--
-info: Try this:
-have fwd : P := rule P (Q ∧ R) h
--/
-#guard_msgs in
-example (rule : ∀ α β, α ∧ β → α) (h : P ∧ Q ∧ R) : P := by
-  forward? [*]
-  guard_hyp fwd : P
-  assumption
-
 /--
 info: Try this:
   have fwd : γ₁ ∧ γ₂ := r₁ a b
   have fwd_1 : δ₁ ∧ δ₂ := r₂ a
+---
+error: unsolved goals
+α : Sort u_1
+β : Sort u_2
+γ₁ γ₂ δ₁ δ₂ : Prop
+a : α
+b : β
+r₁ : α → β → γ₁ ∧ γ₂
+r₂ : α → δ₁ ∧ δ₂
+fwd : γ₁ ∧ γ₂
+fwd_1 : δ₁ ∧ δ₂
+⊢ γ₁ ∧ γ₂ ∧ δ₁ ∧ δ₂
 -/
 #guard_msgs in
 example (a : α) (b : β) (r₁ : (a : α) → (b : β) → γ₁ ∧ γ₂)
     (r₂ : (a : α) → δ₁ ∧ δ₂) : γ₁ ∧ γ₂ ∧ δ₁ ∧ δ₂ := by
   saturate? [*]
-  guard_hyp fwd : γ₁ ∧ γ₂
-  guard_hyp fwd_1 : δ₁ ∧ δ₂
-  aesop
 
 /--
 info: Try this:
   have fwd : β := h₁ h₃
   have fwd_1 : γ := h₂ fwd
+---
+error: unsolved goals
+α β γ : Prop
+h₁ : α → β
+h₂ : β → γ
+h₃ : α
+fwd : β
+fwd_1 : γ
+⊢ γ
 -/
 #guard_msgs in
 example {α β γ : Prop} (h₁ : α → β) (h₂ : β → γ) (h₃ : α) : γ := by
   saturate? [*]
-  guard_hyp fwd : β
-  guard_hyp fwd_1 : γ
-  assumption
 
 /--
 info: Try this:
@@ -170,34 +120,309 @@ fwd_1 : γ
 example {α β γ δ : Prop} (h₁ : α → β) (h₂ : α → γ) (h₃ : β → γ → δ) (h₄ : α) : δ := by
   saturate? 1 [*]
 
+example {P : Nat → Prop} (hP : P 0) (hPn : ∀ n, P n → P (n + 1)) : P 20 := by
+  saturate 20 [*]
+  assumption
+
+section
+
 axiom A : Type
 axiom B : Type
 axiom C : Type
 
-@[aesop safe forward]
+@[local aesop safe forward]
 axiom ab : A → B
 
-@[aesop norm forward]
+@[local aesop norm forward]
 axiom bc : B → C
+
+/--
+info: Try this:
+have fwd : P := rule P (Q ∧ R) h
+-/
+#guard_msgs in
+example (rule : ∀ α β, α ∧ β → α) (h : P ∧ Q ∧ R) : P := by
+  forward? [*]
+  guard_hyp fwd : P
+  assumption
 
 /--
 info: Try this:
   have fwd : B := ab a
   have fwd_1 : C := bc fwd
+---
+error: unsolved goals
+a : A
+fwd : B
+fwd_1 : C
+⊢ C
 -/
 #guard_msgs in
 noncomputable example : A → C := by
   intro a
   saturate?
-  guard_hyp fwd : B
-  guard_hyp fwd_1 : C
-  exact fwd_1
 
-/-! # Tests for Aesop's forward rules -/
+end
+
+/--
+info: Try this:
+have fwd : R a b := h₁ a b h₂ h₃
+---
+error: unsolved goals
+α : Sort u_1
+β : Sort u_2
+a : α
+b : β
+P Q R : α → β → Prop
+h₁ : ∀ (a : α) (b : β), P a b → Q a b → R a b
+h₂ : P a b
+h₃ : Q a b
+fwd : R a b
+⊢ R a b
+-/
+#guard_msgs in
+example {P Q R : α → β → Prop} (h₁ : ∀ a b, P a b → Q a b → R a b)
+    (h₂ : P a b) (h₃ : Q a b) : R a b := by
+  saturate? [h₁]
+
+/--
+info: Try this:
+have fwd : R a b := h₁ a b h₂ h₄
+---
+error: unsolved goals
+α : Sort u_1
+a b : α
+P Q R : α → α → Prop
+h₁ : ∀ (a b : α), P a b → Q b a → R a b
+h₂ : P a b
+h₃ : Q a b
+h₄ : Q b a
+fwd : R a b
+⊢ R a b
+-/
+#guard_msgs in
+example {P Q R : α → α → Prop} (h₁ : ∀ a b, P a b → Q b a → R a b)
+    (h₂ : P a b) (h₃ : Q a b) (h₄ : Q b a) : R a b := by
+  saturate? [*]
+
+/--
+error: unsolved goals
+α : Sort u_1
+a b : α
+P Q R : α → α → Prop
+h₁ : ∀ (a b : α), P a b → Q b a → R a b
+h₂ : P a b
+h₃ : Q a b
+⊢ R a b
+-/
+#guard_msgs in
+example {P Q R : α → α → Prop} (h₁ : ∀ a b, P a b → Q b a → R a b)
+    (h₂ : P a b) (h₃ : Q a b) : R a b := by
+  saturate [*]
+
+/--
+info: Try this:
+have fwd : R b a := h₁ b a h₄ h₃
+---
+error: unsolved goals
+α : Sort u_1
+c d a b : α
+P Q R : α → α → Prop
+h₁ : ∀ (a b : α), P a b → Q b a → R a b
+h₂ : P c d
+h₃ : Q a b
+h₄ : P b a
+fwd : R b a
+⊢ R b a
+-/
+#guard_msgs in
+example {P Q R : α → α → Prop} (h₁ : ∀ a b, P a b → Q b a → R a b)
+    (h₂ : P c d) (h₃ : Q a b) (h₄ : P b a) : R b a := by
+  saturate? [*]
+
+/--
+info: Try this:
+  have fwd : R c c := h₁ c d d c h₂ h₅
+  have fwd_1 : R c b := h₁ c d a b h₂ h₃
+  have fwd_2 : R b c := h₁ b a d c h₄ h₅
+  have fwd_3 : R b b := h₁ b a a b h₄ h₃
+---
+error: unsolved goals
+α : Sort u_1
+c d a b : α
+P Q R : α → α → Prop
+h₁ : ∀ (a b c d : α), P a b → Q c d → R a d
+h₂ : P c d
+h₃ : Q a b
+h₄ : P b a
+h₅ : Q d c
+fwd : R c c
+fwd_1 : R c b
+fwd_2 : R b c
+fwd_3 : R b b
+⊢ R c b
+-/
+#guard_msgs in
+example {P Q R : α → α → Prop} (h₁ : ∀ a b c d, P a b → Q c d → R a d)
+    (h₂ : P c d) (h₃ : Q a b) (h₄ : P b a) (h₅ : Q d c) : R c b := by
+  saturate? [*]
+
+/--
+info: Try this:
+  have fwd : S a d := h₁ a b c d h₂ h₃ h₄
+  have fwd_1 : S a c := h₁ a b d c h₂ h₃ h₅
+---
+error: unsolved goals
+α : Sort u_1
+a b c d : α
+P Q R S : α → α → Prop
+h₁ : ∀ (a b c d : α), P a b → Q b a → R c d → S a d
+h₂ : P a b
+h₃ : Q b a
+h₄ : R c d
+h₅ : R d c
+fwd : S a d
+fwd_1 : S a c
+⊢ S a d
+-/
+#guard_msgs in
+example {P Q R S : α → α → Prop} (h₁ : ∀ a b c d, P a b → Q b a → R c d → S a d)
+    (h₂ : P a b) (h₃ : Q b a) (h₄ : R c d) (h₅ : R d c) : S a d := by
+  saturate? [*]
+
+/--
+info: Try this:
+have fwd : R b a := h₁ a b h₂ h₃ h₄
+---
+error: unsolved goals
+α : Sort u_1
+a b : α
+P : α → Prop
+Q R : α → α → Prop
+h₁ : ∀ (a b : α), P a → P b → Q a b → R b a
+h₂ : P a
+h₃ : P b
+h₄ : Q a b
+fwd : R b a
+⊢ Q b a
+-/
+#guard_msgs in
+example {P : α → Prop} {Q R : α → α → Prop}
+    (h₁ : ∀ a b, P a → P b → Q a b → R b a)
+    (h₂ : P a) (h₃ : P b) (h₄ : Q a b) : Q b a := by
+  saturate? [*]
+
+/--
+info: Try this:
+have fwd : R b a := h₁ a b h₆ h₅ h₄
+---
+error: unsolved goals
+α : Sort u_1
+c d a b : α
+P : α → Prop
+Q R : α → α → Prop
+h₁ : ∀ (a b : α), P a → P b → Q a b → R b a
+h₂ : P c
+h₃ : P d
+h₄ : Q a b
+h₅ : P b
+h₆ : P a
+fwd : R b a
+⊢ Q b a
+-/
+#guard_msgs in
+example {P : α → Prop} {Q R : α → α → Prop}
+    (h₁ : ∀ a b, P a → P b → Q a b → R b a)
+    (h₂ : P c) (h₃ : P d) (h₄ : Q a b) (h₅ : P b) (h₆ : P a) : Q b a := by
+  saturate? [*]
+
+/--
+info: Try this:
+  have fwd : R c d := h₁ d c h₃ h₂ h₇
+  have fwd_1 : R b a := h₁ a b h₆ h₅ h₄
+---
+error: unsolved goals
+α : Sort u_1
+c d a b : α
+P : α → Prop
+Q R : α → α → Prop
+h₁ : ∀ (a b : α), P a → P b → Q a b → R b a
+h₂ : P c
+h₃ : P d
+h₄ : Q a b
+h₅ : P b
+h₆ : P a
+h₇ : Q d c
+fwd : R c d
+fwd_1 : R b a
+⊢ Q b a
+-/
+#guard_msgs in
+example {P : α → Prop} {Q R : α → α → Prop}
+    (h₁ : ∀ a b, P a → P b → Q a b → R b a)
+    (h₂ : P c) (h₃ : P d) (h₄ : Q a b) (h₅ : P b) (h₆ : P a) (h₇ : Q d c) : Q b a := by
+  saturate? [*]
 
 example (a : α) (b : β) (r₁ : (a : α) → (b : β) → γ₁ ∧ γ₂)
     (r₂ : (a : α) → δ₁ ∧ δ₂) : γ₁ ∧ γ₂ ∧ δ₁ ∧ δ₂ := by
   aesop (add safe [forward r₁, forward (immediate := [a]) r₂])
+
+section MatchRedundancy
+
+-- Complete matches are considered redundant (and hence do not produce new
+-- hypotheses) if they agree on all variables that appear in the conclusion.
+
+/--
+error: unsolved goals
+γ : Sort u_1
+α : Prop
+β : Type
+r : α → β → γ
+a₁ a₂ : α
+b₁ b₂ : β
+fwd : γ
+⊢ True
+-/
+#guard_msgs in
+example {α : Prop} {β : Type} (r : α → β → γ) (a₁ a₂ : α) (b₁ b₂ : β) : True := by
+  saturate [r]
+  -- Only one new hypothesis.
+
+/--
+error: unsolved goals
+α : Sort u_1
+a₁ a₂ : α
+P Q : α → Prop
+r : ∀ (a : α), P a → Q a
+p₁ : P a₁
+p₂ p₂' : P a₂
+fwd : Q a₁
+fwd_1 : Q a₂
+⊢ True
+-/
+#guard_msgs in
+example {P Q : α → Prop} (r : ∀ a, P a → Q a) (p₁ : P a₁) (p₂ : P a₂)
+    (p₂' : P a₂) : True := by
+  saturate [r]
+  -- Two new hypotheses, one for `a₁` and one for `a₂` (but not two).
+
+-- When a hypothesis already exists in the context, it is not added again.
+
+/--
+error: unsolved goals
+α : Sort u_1
+β : Sort u_2
+r₁ r₂ : α → β
+a₁ a₂ : α
+fwd : β
+⊢ True
+-/
+#guard_msgs in
+example (r₁ r₂ : α → β) (a₁ a₂ : α) : True := by
+  saturate [r₁, r₂]
+  -- Two new hypotheses (but not four).
+
+end MatchRedundancy
 
 /--
 info: Try this:
@@ -212,15 +437,261 @@ example (a : α) (b : β) (r₁ : (a : α) → (b : β) → γ₁ ∧ γ₂)
     (r₂ : (a : α) → δ₁ ∧ δ₂) : γ₁ ∧ γ₂ ∧ δ₁ ∧ δ₂ := by
   aesop? (add safe [forward r₁, forward (immediate := [a]) r₂])
 
+-- `destruct` rules only clear propositional hypotheses. So this succeeds:
+
+example (a : α) (b : β) (r₁ : (a : α) → (b : β) → γ)
+    (r₂ : (a : α) → δ) : γ ∧ δ := by
+  aesop (add safe [destruct r₁, destruct (immediate := [a]) r₂])
+    (config := { enableSimp := false, terminal := true })
+
+-- ... but this fails:
+
+/-- error: tactic 'aesop' failed, failed to prove the goal after exhaustive search. -/
+#guard_msgs in
+example {α : Prop} (a : α) (b : β) (r₁ : (a : α) → (b : β) → γ)
+    (r₂ : (a : α) → δ) : γ ∧ δ := by
+  aesop (add safe [destruct r₁, destruct (immediate := [a]) r₂])
+    (config := { enableSimp := false, terminal := true })
+
+-- Same examples with `saturate`. Note: We currently can't make local `saturate`
+-- rules into `destruct` rules.
+
+namespace SaturateEx₁
+
+axiom α : Type
+axiom β : Type
+axiom γ₁ : Prop
+axiom γ₂ : Prop
+axiom δ₁ : Prop
+axiom δ₂ : Prop
+@[aesop safe destruct]
+axiom r₁ : α → β → γ₁ ∧ γ₂
+@[aesop safe destruct]
+axiom r₂ : α → δ₁ ∧ δ₂
+
 /--
-error: tactic 'aesop' failed, failed to prove the goal after exhaustive search.
+error: unsolved goals
+a : α
+b : β
+fwd : γ₁ ∧ γ₂
+fwd_1 : δ₁ ∧ δ₂
+⊢ γ₁ ∧ γ₂ ∧ δ₁ ∧ δ₂
 -/
 #guard_msgs in
-example (a : α) (b : β) (r₁ : (a : α) → (b : β) → γ₁ ∧ γ₂)
-    (r₂ : (a : α) → δ₁ ∧ δ₂) : γ₁ ∧ γ₂ ∧ δ₁ ∧ δ₂ := by
-  aesop (add safe [destruct r₁, destruct (immediate := [a]) r₂])
-    (config := { terminal := true })
+example (a : α) (b : β) : γ₁ ∧ γ₂ ∧ δ₁ ∧ δ₂ := by
+  saturate
+
+end SaturateEx₁
+
+namespace SaturateEx₂
+
+axiom α : Prop
+axiom β : Type
+axiom γ₁ : Prop
+axiom γ₂ : Prop
+axiom δ₁ : Prop
+axiom δ₂ : Prop
+@[aesop safe destruct]
+axiom r₁ : α → β → γ₁ ∧ γ₂
+@[aesop safe destruct]
+axiom r₂ : α → δ₁ ∧ δ₂
+
+/--
+error: unsolved goals
+b : β
+fwd : γ₁ ∧ γ₂
+⊢ γ₁ ∧ γ₂ ∧ δ₁ ∧ δ₂
+-/
+#guard_msgs in
+example (a : α) (b : β) : γ₁ ∧ γ₂ ∧ δ₁ ∧ δ₂ := by
+  saturate
+
+end SaturateEx₂
 
 example (a : α) (b : β) (r₁ : (a : α) → (b : β) → γ₁ ∧ γ₂)
     (r₂ : (a : α) → δ₁ ∧ δ₂) : γ₁ ∧ γ₂ ∧ δ₁ ∧ δ₂ := by
   aesop (add safe [forward r₁], 90% destruct r₂)
+
+/--
+warning: aesop: failed to prove the goal after exhaustive search.
+---
+error: unsolved goals
+α β γ : Prop
+h₁ : α
+h₂ : β
+fwd : γ
+⊢ False
+-/
+#guard_msgs in
+example {α β γ : Prop} (h : α → β → γ) (h₁ : α) (h₂ : β) : False := by
+  aesop (add norm -1 forward h)
+
+-- In the following example, `h` does not apply because `simp_all` discharges
+-- the premises `α` and `β`. The stateful implementation of forward reasoning
+-- can't reasonably deal with local rules whose types change during the course
+-- of the search; the best we can do is try to detect when this happens.
+
+/--
+warning: aesop: failed to prove the goal after exhaustive search.
+---
+error: unsolved goals
+α β γ : Prop
+h : γ
+h₁ : α
+h₂ : β
+⊢ False
+-/
+#guard_msgs in
+example {α β γ : Prop} (h : α → β → γ) (h₁ : α) (h₂ : β) : False := by
+  aesop (add safe forward h)
+
+section Computation
+
+-- Stateful forward reasoning sees through `reducible` definitions...
+
+abbrev rid (x : α) : α := x
+
+example {P Q : α → Prop} (h₁ : ∀ a, P a → Q a → X) (h₂ : P (rid a)) (h₃ : Q a) : X := by
+  saturate [h₁]
+  exact fwd
+
+-- ... but not through semireducible ones.
+
+/--
+error: unsolved goals
+α : Sort _
+X : Sort _
+a : α
+P Q : α → Prop
+h₁ : (a : α) → P a → Q a → X
+h₂ : P (id a)
+h₃ : Q a
+⊢ X
+-/
+#guard_msgs in
+example {P Q : α → Prop} (h₁ : ∀ a, P a → Q a → X) (h₂ : P (id a)) (h₃ : Q a) : X := by
+  saturate [h₁]
+
+end Computation
+
+namespace Immediate
+
+axiom α : Type
+axiom P : α → Prop
+axiom Q : α → Prop
+axiom R : α → Prop
+
+@[aesop safe forward (immediate := [h₂])]
+axiom foo : ∀ a (h₁ : P a) (h₂ : Q a), R a
+
+/--
+error: unsolved goals
+a : α
+h : Q a
+fwd : P a → R a
+⊢ False
+-/
+#guard_msgs in
+example (h : Q a) : False := by
+  saturate
+
+end Immediate
+
+namespace Instance
+
+class Foo (α : Type) : Prop
+
+axiom β : Type
+
+@[aesop safe forward]
+axiom foo : ∀ (α : Type) (a : α) [Foo α], β
+
+/--
+error: unsolved goals
+α : Type
+inst✝ : Foo α
+a : α
+fwd : β
+⊢ False
+-/
+#guard_msgs in
+example [Foo α] (a : α) : False := by
+  saturate
+
+axiom γ : Type
+
+instance : Foo γ where
+
+/--
+error: unsolved goals
+c : γ
+fwd : β
+⊢ False
+-/
+#guard_msgs in
+example (c : γ) : False := by
+  saturate
+
+@[aesop safe forward (immediate := [a])]
+axiom bar : ∀ α β (a : α) (b : β) [Foo β], γ
+
+/--
+error: unsolved goals
+α : Sort u_1
+a : α
+⊢ False
+-/
+#guard_msgs in
+example (a : α) : False := by
+  saturate
+
+/--
+error: unsolved goals
+c : γ
+fwd : β
+⊢ False
+-/
+#guard_msgs in
+example (c : γ) : False := by
+  saturate
+
+end Instance
+
+namespace ConstForwardRule
+
+axiom α : Type
+@[local aesop safe forward]
+axiom a : α
+
+noncomputable example : α := by
+  aesop
+
+/--
+error: unsolved goals
+fwd : α
+⊢ α
+-/
+#guard_msgs in
+noncomputable example : α := by
+  saturate
+
+end ConstForwardRule
+
+section MultipleUniverses
+
+-- Here we test the handling of rules with multiple universe parameters.
+
+axiom α.{u} : Type u
+axiom β.{v} : Type v
+axiom γ.{w} : Type w
+axiom P.{u, v, w} : α.{u} → β.{v} → γ.{w} → Prop
+axiom Q.{u, v, w} : β.{v} → α.{u} → γ.{w} → Prop
+
+@[local aesop safe forward]
+axiom foo {a b c} : P a b c → Q b a c
+
+example (h : P a b c) : Q b a c := by
+  saturate
+  assumption
+
+end MultipleUniverses
