Aesop/BuiltinRules/ApplyHyps.lean
@@ -12,11 +12,11 @@ open Lean
 open Lean.Meta
 
 def applyHyp (hyp : FVarId) (goal : MVarId) (md : TransparencyMode) :
-    MetaM RuleApplication := do
+    BaseM RuleApplication := do
   let (goals, #[step]) ← applyS goal (.fvar hyp) none md |>.run
     | throwError "aesop: internal error in applyHyps: multiple steps"
   return {
-    goals := goals.map ({ mvarId := ·, diff := ∅ })
+    goals := goals.map λ mvarId => { diff := .empty goal mvarId }
     postState := step.postState
     scriptSteps? := #[step]
     successProbability? := none
