Aesop/Forward/State/ApplyGoalDiff.lean
@@ -1,0 +1,59 @@
+/-
+Copyright (c) 2024 Jannis Limperg. All rights reserved.
+Released under Apache 2.0 license as described in the file LICENSE.
+Authors: Jannis Limperg
+-/
+
+import Aesop.Forward.State
+import Aesop.RuleSet
+
+namespace Aesop
+
+open Lean Lean.Meta
+
+/-- Apply a goal diff to the state, adding and removing hypotheses as indicated
+by the diff. -/
+def ForwardState.applyGoalDiff (rs : LocalRuleSet) (diff : GoalDiff)
+    (fs : ForwardState) : BaseM (ForwardState × Array ForwardRuleMatch) := do
+  if ! aesop.dev.statefulForward.get (← getOptions) then
+    -- We still update the hyp types since these are also used by stateless
+    -- forward reasoning.
+    return ({ fs with hypTypes := ← updateHypTypes fs.hypTypes } , #[])
+  let fs ← diff.oldGoal.withContext do
+    diff.removedFVars.foldM (init := fs) λ fs h => do eraseHyp h fs
+  diff.newGoal.withContext do
+    let (fs, ruleMatches) ←
+      diff.addedFVars.foldM (init := (fs, ∅)) λ (fs, ruleMatches) h => do
+        addHyp h fs ruleMatches
+    if ← diff.targetChanged' then
+      updateTarget fs ruleMatches
+    else
+      return (fs, ruleMatches)
+where
+  eraseHyp (h : FVarId) (fs : ForwardState) : BaseM ForwardState :=
+    return fs.eraseHyp h (← rpinf (← h.getType))
+
+  addHyp (h : FVarId) (fs : ForwardState)
+      (ruleMatches : Array ForwardRuleMatch) :
+      BaseM (ForwardState × Array ForwardRuleMatch) := do
+    let rules ← rs.applicableForwardRules (← h.getType)
+    let patInsts ← rs.forwardRulePatternSubstsInLocalDecl (← h.getDecl)
+    fs.addHypWithPatSubstsCore ruleMatches diff.newGoal h rules patInsts
+
+  updateTarget (fs : ForwardState) (ruleMatches : Array ForwardRuleMatch) :
+      BaseM (ForwardState × Array ForwardRuleMatch) := do
+    let patInsts ←
+      rs.forwardRulePatternSubstsInExpr (← diff.newGoal.getType)
+    fs.updateTargetPatSubstsCore ruleMatches diff.newGoal patInsts
+
+  updateHypTypes (hypTypes : PHashSet RPINF) : BaseM (PHashSet RPINF) := do
+    let mut hypTypes := hypTypes
+    for fvarId in diff.removedFVars do
+      let type ← diff.oldGoal.withContext do rpinf (← fvarId.getType)
+      hypTypes := hypTypes.erase type
+    for fvarId in diff.addedFVars do
+      let type ← diff.newGoal.withContext do rpinf (← fvarId.getType)
+      hypTypes := hypTypes.insert type
+    return hypTypes
+
+end Aesop
