Aesop/Index/RulePattern.lean
@@ -1,0 +1,164 @@
+/-
+Copyright (c) 2024 Jannis Limperg. All rights reserved.
+Released under Apache 2.0 license as described in the file LICENSE.
+Authors: Jannis Limperg
+-/
+
+import Aesop.Index.Basic
+import Aesop.RuleTac.GoalDiff
+import Batteries.Lean.Meta.DiscrTree
+
+set_option linter.missingDocs true
+
+open Lean Lean.Meta
+
+namespace Aesop
+
+/-- A map from rule names to rule pattern substitutions. When run on a goal,
+the rule pattern index returns such a map. -/
+abbrev RulePatternSubstMap := Std.HashMap RuleName (Std.HashSet Substitution)
+
+namespace RulePatternSubstMap
+
+/-- Insert an array of rule pattern substitutions into a rule pattern
+substitution map. -/
+def insertArray (xs : Array (RuleName × Substitution))
+    (m : RulePatternSubstMap) : RulePatternSubstMap :=
+  xs.foldl (init := m) λ m (r, inst) =>
+    match m[r]? with
+    | none => m.insert r $ (∅ : Std.HashSet _).insert inst
+    | some insts => m.insert r $ insts.insert inst
+
+/-- Build a rule pattern substitution map from an array of substitutions. -/
+def ofArray (xs : Array (RuleName × Substitution)) : RulePatternSubstMap :=
+  (∅ : RulePatternSubstMap).insertArray xs
+
+/-- Convert a rule pattern substitution map to a flat array of substitutions. -/
+def toFlatArray (m : RulePatternSubstMap) : Array (RuleName × Substitution) :=
+  m.fold (init := #[]) λ acc r patInsts =>
+    patInsts.fold (init := acc) λ acc patInst =>
+      acc.push (r, patInst)
+
+end RulePatternSubstMap
+
+
+/-- An entry of the rule pattern index. -/
+structure RulePatternIndex.Entry where
+  /-- The name of the rule to which the pattern belongs. -/
+  name : RuleName
+  /-- The rule's pattern. We assume that there is at most one pattern per
+  rule. -/
+  pattern : RulePattern
+  deriving Inhabited
+
+instance : BEq RulePatternIndex.Entry where
+  beq e₁ e₂ := e₁.name == e₂.name
+
+set_option linter.missingDocs false in
+/-- A rule pattern index. Maps expressions `e` to rule patterns that likely
+unify with `e`. -/
+structure RulePatternIndex where
+  /-- The index. -/
+  tree : DiscrTree RulePatternIndex.Entry
+  /-- `true` iff the index contains no patterns. -/
+  isEmpty : Bool
+  deriving Inhabited
+
+namespace RulePatternIndex
+
+instance : EmptyCollection RulePatternIndex :=
+  ⟨⟨{}, true⟩⟩
+
+/-- Add a rule pattern to the index. -/
+def add (name : RuleName) (pattern : RulePattern) (idx : RulePatternIndex) :
+    RulePatternIndex :=
+  ⟨idx.tree.insertCore pattern.discrTreeKeys { name, pattern }, false⟩
+
+/-- Merge two rule pattern indices. Patterns that appear in both indices appear
+twice in the result. -/
+def merge (idx₁ idx₂ : RulePatternIndex) : RulePatternIndex :=
+  if idx₁.isEmpty then
+    idx₂
+  else if idx₂.isEmpty then
+    idx₁
+  else
+    ⟨idx₁.tree.mergePreservingDuplicates idx₂.tree, false⟩
+
+section Get
+
+/-- Get rule pattern substitutions for the patterns that match `e`. -/
+def getSingle (e : Expr) (idx : RulePatternIndex) :
+    BaseM (Array (RuleName × Substitution)) := do
+  if idx.isEmpty then
+    return #[]
+  let ms ← getUnify idx.tree e
+  ms.filterMapM λ { name := r, pattern } => do
+    let some subst ← pattern.match e
+      | return none
+    return (r, subst)
+
+/-- Get all substitutions of the rule patterns that match a subexpression of
+`e`. Subexpressions containing bound variables are not considered. The returned
+array may contain duplicates. -/
+def getCore (e : Expr) (idx : RulePatternIndex) :
+    BaseM (Array (RuleName × Substitution)) := do
+  if idx.isEmpty then
+    return #[]
+  let e ← instantiateMVars e
+  checkCache (β := RulePatternCache.Entry) e λ _ => do
+    let (_, ms) ← e.forEach getSubexpr |>.run #[]
+    return ms
+where
+  getSubexpr (e : Expr) :
+      StateRefT (Array (RuleName × Substitution)) BaseM Unit := do
+    if e.hasLooseBVars then
+      -- We don't visit subexpressions with loose bvars. Substitutions
+      -- derived from such subexpressions would not be valid in the goal's
+      -- context. E.g. if a rule `(x : T) → P x` has pattern `x` and we
+      -- have the expression `λ (y : T), y` in the goal, then it makes no
+      -- sense to match `y` and generate `P y`.
+      return
+    let ms ← idx.getSingle e
+    modifyThe (Array _) (· ++ ms)
+
+@[inherit_doc getCore]
+def get (e : Expr) (idx : RulePatternIndex) : BaseM RulePatternSubstMap :=
+  .ofArray <$> idx.getCore e
+
+/-- Get all substitutions of the rule patterns that match a subexpression of
+the given local declaration. Subexpressions containing bound variables are not
+considered. -/
+def getInLocalDeclCore (acc : RulePatternSubstMap) (ldecl : LocalDecl)
+    (idx : RulePatternIndex) : BaseM RulePatternSubstMap := do
+  if idx.isEmpty then
+    return acc
+  let mut result := acc
+  result := result.insertArray $ ← idx.getCore ldecl.toExpr
+  result := result.insertArray $ ← idx.getCore ldecl.type
+  if let some val := ldecl.value? then
+    result := result.insertArray $ ← idx.getCore val
+  return result
+
+@[inherit_doc getInLocalDeclCore]
+def getInLocalDecl (ldecl : LocalDecl) (idx : RulePatternIndex) :
+    BaseM RulePatternSubstMap :=
+  idx.getInLocalDeclCore ∅ ldecl
+
+/-- Get all substitutions of the rule patterns that match a subexpression of
+a hypothesis or the target. Subexpressions containing bound variables are not
+considered. -/
+def getInGoal (goal : MVarId) (idx : RulePatternIndex) :
+    BaseM RulePatternSubstMap :=
+  goal.withContext do
+    if idx.isEmpty then
+      return ∅
+    let mut result := ∅
+    for ldecl in (← goal.getDecl).lctx do
+      unless ldecl.isImplementationDetail do
+        result ← idx.getInLocalDeclCore result ldecl
+    result := result.insertArray $ ← idx.getCore (← goal.getType)
+    return result
+
+end Get
+
+end Aesop.RulePatternIndex
