Aesop/RPINF/Basic.lean
@@ -1,0 +1,145 @@
+/-
+Copyright (c) 2024 Jannis Limperg. All rights reserved.
+Released under Apache 2.0 license as described in the file LICENSE.
+Authors: Jannis Limperg
+-/
+
+import Lean
+
+set_option linter.missingDocs true
+
+open Lean Lean.Meta
+
+namespace Aesop
+
+/-- `MData` tag for expressions that are proofs. -/
+def mdataPINFIsProofName : Name :=
+  `Aesop.pinfIsProof
+
+/-- Modify `d` to indicate that the enclosed expression is a proof. -/
+def mdataSetIsProof (d : MData) : MData :=
+  d.insert mdataPINFIsProofName true
+
+/-- Check whether `d` indicates that the enclosed expression is a proof. -/
+def mdataIsProof (d : MData) : Bool :=
+  d.getBool mdataPINFIsProofName (defVal := false)
+
+mutual
+  /-- Check whether two expressions in PINF are equal. We assume that the two
+  expressions are type-correct, in PINF and have defeq types. -/
+  def pinfEqCore : (x y : Expr) → Bool
+    | .bvar i₁, .bvar i₂ => i₁ == i₂
+    | .fvar id₁, .fvar id₂ => id₁ == id₂
+    | .mvar id₁, .mvar id₂ => id₁ == id₂
+    | .sort u, .sort v => u == v
+    | .const n₁ us, .const n₂ vs => n₁ == n₂ && us == vs
+    | .app f₁ e₁, .app f₂ e₂ => pinfEq f₁ f₂ && pinfEq e₁ e₂
+    | .lam _ t₁ e₁ bi₁, .lam _ t₂ e₂ bi₂ =>
+      bi₁ == bi₂ && pinfEq t₁ t₂ && pinfEq e₁ e₂
+    | .forallE _ t₁ e₁ bi₁, .forallE _ t₂ e₂ bi₂ =>
+      bi₁ == bi₂ && pinfEq t₁ t₂ && pinfEq e₁ e₂
+    | .letE _ t₁ v₁ e₁ _, .letE _ t₂ v₂ e₂ _ =>
+      pinfEq v₁ v₂ && pinfEq t₁ t₂ && pinfEq e₁ e₂
+    | .lit l₁, .lit l₂ => l₁ == l₂
+    | .mdata d e₁, e₂ | e₁, .mdata d e₂ => mdataIsProof d || pinfEq e₁ e₂
+    | _, _ => false
+
+  @[inherit_doc pinfEqCore]
+  def pinfEq (x y : Expr) : Bool :=
+    (unsafe ptrEq x y) || pinfEqCore x y
+end
+
+/-- Compute the PINF hash of an expression in PINF. The hash ignores binder
+names, binder info and proofs marked by `mdataPINFIsProofName`. -/
+partial def pinfHashCore (e : Expr) :
+    StateRefT (Std.HashMap UInt64 UInt64) (ST s) UInt64 :=
+  have : MonadHashMapCacheAdapter UInt64 UInt64
+           (StateRefT (Std.HashMap UInt64 UInt64) (ST s)) := {
+    getCache := get
+    modifyCache := modify
+  }
+  checkCache e.hash λ _ => do
+    match e with
+    | .app .. =>
+      let h ← pinfHashCore e.getAppFn
+      e.getAppArgs.foldlM (init := h) λ h arg =>
+        return mixHash h (← pinfHashCore arg)
+    | .lam _ t b _ | .forallE _ t b _ =>
+      return mixHash (← pinfHashCore t) (← pinfHashCore b)
+    | .letE _ t v b _ =>
+      return mixHash (← pinfHashCore t) $
+        mixHash (← pinfHashCore v) (← pinfHashCore b)
+    | .proj t i e =>
+      return mixHash (← pinfHashCore e) $ mixHash (hash t) (hash i)
+    | .mdata d e => if mdataIsProof d then return 13 else pinfHashCore e
+    | .sort .. | .mvar .. | .lit .. | .const .. | .fvar .. | .bvar .. =>
+      return e.hash
+
+@[inherit_doc pinfHashCore]
+def pinfHash (e : Expr) : UInt64 :=
+  runST λ _ => pinfHashCore e |>.run' ∅
+
+set_option linter.missingDocs false in
+/-- An expression in PINF at transparency `md`. -/
+structure PINFRaw (md : TransparencyMode) where
+  toExpr : Expr
+  deriving Inhabited
+
+instance : BEq (PINFRaw md) where
+  beq x y := pinfEq x.toExpr y.toExpr
+
+instance : Hashable (PINFRaw md) where
+  hash x := pinfHash x.toExpr
+
+instance : ToString (PINFRaw md) where
+  toString x := toString x.toExpr
+
+instance : ToFormat (PINFRaw md) where
+  format x := format x.toExpr
+
+instance : ToMessageData (PINFRaw md) where
+  toMessageData x := toMessageData x.toExpr
+
+/-- An expression in PINF at `reducible` transparency. -/
+abbrev RPINFRaw := PINFRaw .reducible
+
+set_option linter.missingDocs false in
+/-- Cache for `rpinf`. -/
+structure RPINFCache where
+  map : Std.HashMap Expr RPINFRaw
+  deriving Inhabited
+
+instance : EmptyCollection RPINFCache :=
+  ⟨⟨∅⟩⟩
+
+set_option linter.missingDocs false in
+/-- An expression in PINF at transparency `md`, together with its PINF hash as
+computed by `pinfHash`. -/
+structure PINF (md : TransparencyMode) where
+  toExpr : Expr
+  hash : UInt64
+  deriving Inhabited
+
+instance : BEq (PINF md) where
+  beq x y := pinfEq x.toExpr y.toExpr
+
+instance : Hashable (PINF md) where
+  hash x := x.hash
+
+instance : Ord (PINF md) where
+  compare x y :=
+    if x == y then .eq else if x.toExpr.lt y.toExpr then .lt else .gt
+
+instance : ToString (PINF md) where
+  toString x := toString x.toExpr
+
+instance : ToFormat (PINF md) where
+  format x := format x.toExpr
+
+instance : ToMessageData (PINF md) where
+  toMessageData x := toMessageData x.toExpr
+
+/-- An expression in RPINF together with its RPINF hash. -/
+abbrev RPINF := PINF .reducible
+
+end Aesop
