Aesop/RuleTac/RuleTerm.lean
@@ -1,0 +1,51 @@
+import Aesop.Rule.Name
+
+open Lean Lean.Meta
+
+namespace Aesop
+
+inductive RuleTerm
+  | const (decl : Name)
+  | term (term : Term)
+  deriving Inhabited
+
+instance : ToMessageData RuleTerm where
+  toMessageData
+    | .const decl => m!"{decl}"
+    | .term tm => m!"{tm}"
+
+inductive ElabRuleTerm
+  | const (decl : Name)
+  | term (term : Term) (expr : Expr)
+  deriving Inhabited
+
+namespace ElabRuleTerm
+
+instance : ToMessageData ElabRuleTerm where
+  toMessageData
+    | .const decl => m!"{decl}"
+    | .term tm _ => m!"{tm}"
+
+def expr : ElabRuleTerm → MetaM Expr
+  | const decl => mkConstWithFreshMVarLevels decl
+  | term _ e => return e
+
+def scope : ElabRuleTerm → ScopeName
+  | const .. => .global
+  | term .. => .local
+
+def name : ElabRuleTerm → MetaM Name
+  | const decl => return decl
+  | term _ e => getRuleNameForExpr e
+
+def toRuleTerm : ElabRuleTerm → RuleTerm
+  | const decl => .const decl
+  | term t _ => .term t
+
+def ofElaboratedTerm (tm : Term) (expr : Expr) : ElabRuleTerm :=
+  if let some decl := expr.constName? then
+    .const decl
+  else
+    .term tm expr
+
+end Aesop.ElabRuleTerm
